---
creation_date: 2024-02-11 14:02
tags:
  - MAAM
share: true
---

$$\begin{gather}
W = 0 = \sum_{k=1}^{n}F_{k}v_{k}+\sum_{k=1}^{n}C_{k}\omega_{k} + \sum_{k=1}^{n}F_{ik}v_{ik}+\sum_{k=1}^{n}C_{ik}\omega_{ik} \\
m_{eq}\ddot{x_{p_{1}}} + r_{eq}\dot{x_{p_{1}}}+k_{eq}x_{p_{1}} = F(t) \\
X_{o} = \frac{F_{o}}{\sqrt{ (k_{eq}-m_{eq}\Omega^{2})^{2}+(r_{eq}\Omega)^{2} }}\\
w_{o} = \sqrt{ \frac{k_{eq}}{m_{eq}} } \\
h = \frac{r_{eq}}{r_{c}} = \frac{r_{eq}}{2m_{eq}w_{o}} \\
a = \frac{\Omega}{\omega_{o}} \\
C_{rR} =uN =f_{v}RN \\
\text{A condizioni di limite: } T = f_{a}N \text{ o } T = f_{d}N \\
a = \dot{\omega}\times R-\omega^{2} R+a_{co}\\
a_{co} = 2 w\times v_{rel} \\
|X(a)| = \frac{X_{st}}{\sqrt{ (1-a^{2})^{2}+(2ah)^{2} }} = X_{st}\cdot H(a  )\\
v = \omega R = |\dot{\theta}|R\\
x = \theta R\\
\frac{d}{dt}\frac{ \partial E_{c} }{ \partial \dot{q}_{i} } - \frac{ \partial E_{c} }{ \partial q_{i} } + \frac{ \partial D }{ \partial q_{i} }   +\frac{ \partial V }{ \partial q_{i} } = \frac{\delta L_{i}}{\delta q_{i}} \\
V = \frac{1}{2}k\Delta l ^{2} +Mgh\\
D = \frac{1}{2}r \dot{\Delta l} ^{2} \\
J_{GL} = \frac{mL^{2}}{12} \\
J_{GiG} = m_{i}|G_{i}-G|^{2} \\
J_{0} = n(J_{GL}+J_{GiG}) + M\overline{OG}^{2}  \\
C_{m} = C_{o}\left( 1-\frac{w_{m}}{w_{s}} \right) \\
\eta_{d} \text{ if } \Pi_{e}>\Pi_{u} \\
\text{elif } \Pi_{e}<\Pi_{u} \implies  \eta_{r} \\
\Omega(R\pm r) = \omega r
\end{gather}$$
 