---
creation_date: 2025-04-03
tags: 
parent: 
child: 
share: false
---
$$\begin{align}
&\rho_{in}v_{m,in}S_{in} = \rho_{out}v_{m,out}S_{out} \to \text{Mass Balance} \\
&\dot{m}\left[\Delta h + \frac{\Delta v^{2}}{2}+g\Delta z\right] = \dot{L}+\dot{Q}\to \text{Total Energy Balance} \\
&T_{i} = \frac{P_{i}}{\rho}+\frac{v_{i}^{2}}{2}+gz_{i}\to \text{Bernoulli Trinomial} \\
&l-l_{w} = \Delta T \to \text{Mechanical Energy Balance}\\
&q+l_{w} = \int\limits_{}^{} T \, ds \\
&\dot{L} = l\cdot \dot{m} \\
&\vec{v} = \vec{u}+\vec{w}\to l = u_{2}v_{2t}-u_{1}v_{1t} =\frac{\Delta v^{2}}{2}-\frac{\Delta w^{2}}{2}+\frac{\Delta u^{2}}{2} \\
&\vec{u} = \frac{2\pi}{60}n\cdot \frac{D}{2} \\
&l-l_{w}-y =\Delta T \\
&y =\sum y_{ci}+y_{_{DISi}} = \sum\xi_{i} \frac{v_{i}^{2}}{2} + \frac{\lambda_{i}L_{i}}{D_{i}}\cdot \frac{v_{i}^{2}}{2} \\
&P_{Ti} = \frac{P_{i}}{\rho} + \frac{v_{i}^{2}}{2} \\
&Q = \rho \cdot \dot{m}   = \frac{\pi D_{i}^{2}v_{i}}{4} \\
&\psi = \frac{gH}{n^{2}D^{2}}\;;\; \varphi = \frac{Q}{nD^{3}} \;;\;\eta = \frac{gH}{l} \\
&\text{Perfect Liquid}\to q+l_{w} = c_{L}\Delta T \\
&gH_{p} = \Delta T_{p} = l-l_{w} \\
&NPSH_{H} = \frac{P_{1}}{\rho g} + \frac{v_{1}^{2}}{2g}-\frac{P_{min}}{\rho g} \\
&NPSH_{A} = \frac{P_{1}}{\rho}+\frac{v_{1}^{2}}{2g}- \frac{P_{SAT}+P_{DIS}}{\rho g} \\
&\text{Avoid Cavitation} \implies  NPSH_{A}>NPSH_{R} \\
&\chi = \frac{P_{2}-P_{1}}{\rho gH} = 1-\frac{v_{2t}}{2u_{2}} \\
&H_{p} = A\left( \frac{\overline{D}_{}}{D} \right)^{4}Q^{2} + B\left( \frac{n}{\overline{n}_{} } \right)\left( \frac{\overline{D}_{}}{D} \right)Q + C\left( \frac{n}{\overline{n}_{} } \right)^{2}\left( \frac{D}{\overline{D}_{} } \right)^{2} \\
&\eta_{p} = E\left( \frac{\overline{n}_{}}{n}  \right)^{2}\left( \frac{\overline{D}_{}}{D} \right)^{6}Q^{2}+ F\left( \frac{\overline{n}_{}}{n} \right)\left( \frac{\overline{D}_{}}{D} \right)^{3}Q+G \\
&\overline{n}_{},\overline{D}\to \text{inital condition}  \;;\;n,D \to \text{New condition} \\
&\dot{L} = \frac{\rho QH}{\eta}g \\
&\text{Serie: }H_{eq} = H_{1}+H_{2}\;\;;\;\;Q_{eq} = Q_{1}=Q_{2} \\
&\text{Parallelo: }H_{eq} = H_{1}=H_{2}\;\;;\;\; Q_{eq} = Q_{1}+Q_{2} \\
&gH_{m} = T_{0}-T_{B} = g(z_{D}-z_{B})-y_{p} \\
&NPSH_{A,\text{turb}} = \frac{P_{2}}{\rho g}+\frac{v_{2}^{2}}{2g}-\frac{P_{sat}+P_{dis}}{\rho g} \\
&v_{1} = \varphi v_{1}'\;\;;\;\;v_{1}' = \sqrt{ 2gH_{m} }\;\;;\;\;w_{2}=\psi w_{1}\;\;;\;\;k_{p} = \frac{u}{v_{1}'} \\
&\eta = 0\text{ if }k_{p}=\varphi,\;\;\eta_{_{BEP}} @ k_{p} = \frac{\varphi}{2}
\end{align}$$
